src/FP/Classes/Monad.v
@@ -1,9 +1,27 @@
 Require Import FP.Data.WeakSetoid.
+Require Import FP.Classes.WeakEqv.
+Require Import FP.Data.Function_Q.
 Require Import FP.Data.Unit.
+Require Import FP.Data.Function.
 
-Import WeakEqv.Notation.
+Import Eqv.Notation.
 Import WeakSetoid.Notation.
 Import Unit.Notation.
+Import Function.Notation.
+Import WeakEqv.Notation.
+
+Definition bind_associativity_k 
+  {m:WeakSetoid -> WeakSetoid} (bind:forall {A B:WeakSetoid}, DD (m A ⇨ (A ⇨ m B) ⇨ m B)) 
+  {A B C:WeakSetoid} (f:DD (A ⇨ m B)) (g:DD (B ⇨ m C))
+  : DD (A ⇨ m C) := 
+    mk_DD_infer (A ⇨ m C) 
+                (fun x => DD_value bind (DD_value f x) (DD_value g)).
+
+(* consider changing A ⇨ B to have DD A -> DD B as underlying type,
+   rather than A -> B.  This is so arbitrary contexts (like the one
+   created above, fun x => DD_value bind ...)  can give good beta
+   rules.  After thinking about it, this sounds like the right way to
+   go, and doesn't contradict anything I've built so far. *)
 
 Class Monad (m:WeakSetoid -> WeakSetoid) : Type :=
   { ret : 
@@ -13,10 +31,14 @@ Class Monad (m:WeakSetoid -> WeakSetoid) : Type :=
       DD (m A ⇨ (A ⇨ m B) ⇨ m B)
   ; monad_left_unit : 
       forall {A:WeakSetoid} (xM:DD (m A)), 
-      bind ⊛ xM ⊛ ret ≈ xM
+      bind ⊛ xM ⊛ ret ≃ xM
   ; monad_right_unit : 
       forall {A B:WeakSetoid} (x:DD A) (k:DD (A ⇨ m B)), 
-      bind ⊛ (ret ⊛ x) ⊛ k ≈ k ⊛ x
+      bind ⊛ (ret ⊛ x) ⊛ k ≃ k ⊛ x
+  ; monad_associativity :
+      forall {A B C:WeakSetoid} (xM:DD (m A)) (f:DD (A ⇨ m B)) (g:DD (B ⇨ m C)),
+      bind ⊛ (bind ⊛ xM ⊛ f) ⊛ g 
+      ≃ bind ⊛ xM ⊛ bind_associativity_k (@bind) f g
   }.
 
 Class MonadState (S:WeakSetoid) (m:WeakSetoid -> WeakSetoid) : Type :=
@@ -30,5 +52,5 @@ Class MonadPlus (m:WeakSetoid -> WeakSetoid) `{! Monad m } : Type :=
       DD (m A ⇨ m A ⇨ m A) 
   ; monad_plus_distributivity : 
       forall {A B:WeakSetoid} (xM yM:DD (m A)) (k:DD (A ⇨ m B)), 
-      bind ⊛ (mplus ⊛ xM ⊛ yM) ⊛ k ≈ mplus ⊛ (bind ⊛ xM ⊛ k) ⊛ (bind ⊛ yM ⊛ k)
+      extend ⊛ k ⊛ (mplus ⊛ xM ⊛ yM) ≃ mplus ⊛ (extend ⊛ k ⊛ xM) ⊛ (extend ⊛ k ⊛ yM)
   }.
