src/FP/Data/RewriteState.v
@@ -5,6 +5,8 @@ Require Import FP.Classes.Symmetric.
 Require Import FP.Classes.Transitive.
 Require Import FP.Data.Relation.
 Require Import FP.Data.Function.
+Require Import FP.Data.Function_Q.
+Require Import FP.Data.Tactic.
 
 Import WeakSetoid.Notation.
 Import WeakEqv.Notation.
@@ -12,84 +14,17 @@ Import Eqv.Notation.
 
 Create HintDb rewrite_beta.
 
-(* Also make this a definition := it's interp, constructors are just opaque things *)
-Inductive RewriteContext : WeakSetoid -> WeakSetoid -> Type :=
-  | RCTop : forall {A}, RewriteContext A A
-  | RCFocusFun : 
-      forall {A B C:WeakSetoid}, 
-      RewriteContext B C -> DD A -> RewriteContext (A ⇨ B) C
-  | RCFocusArg : 
-      forall {A B C:WeakSetoid}, 
-      RewriteContext B C -> DD (A ⇨ B) -> RewriteContext A C.
-Arguments RCTop {A}.
-Arguments RCFocusFun {A B C} _ _.
-Arguments RCFocusArg {A B C} _ _.
-
-Definition rewrite_context_interp {A B:WeakSetoid} (e:DD A) (k:RewriteContext A B) : DD B.
-Proof.
-  induction k ; auto. 
-  apply IHk ; exact (e ⊛ d).
-  apply IHk ; exact (d ⊛ e).
-Defined.
-
-Definition rewrite_context_respect_weqv 
-  {A B:WeakSetoid} 
-  (x y:DD A) (p:x ≃ y) (rc:RewriteContext A B) 
-  : rewrite_context_interp x rc ≃ rewrite_context_interp y rc.
-Proof.
-  induction rc ; simpl in * ; auto.
-  - apply IHrc ; decide_weqv.
-  - apply IHrc ; decide_weqv.
-Defined.
-
+Definition RewriteContext (A B:WeakSetoid) := DD (A ⇨ B).
+Definition RCTop {A:WeakSetoid} : RewriteContext A A := id_Q.
+Definition RCFocusFun {A B C:WeakSetoid} (k:DD (B ⇨ C)) (x:DD A) : RewriteContext (A ⇨ B) C :=
+  compose_Q ⊛ k ⊛ (apply_to_Q ⊛ x).
+Definition RCFocusArg {A B C:WeakSetoid} (k:DD (B ⇨ C)) (f:DD (A ⇨ B)) : RewriteContext A C :=
+  compose_Q ⊛ k ⊛ (apply_Q ⊛ f).
+                                                              
 Definition RewriteState 
-  {A B:WeakSetoid} 
-  (e:DD A) (k:RewriteContext A B) (g:DD B) : Type := rewrite_context_interp e k ≃ g.
-Definition mk_RewriteState 
-  {A B:WeakSetoid}
-  (e:DD A) (k:RewriteContext A B) (g:DD B) 
-  (p:rewrite_context_interp e k ≃ g)
-  : RewriteState e k g := p.
-Definition un_RewriteState 
-  {A B:WeakSetoid}
-  (e:DD A) (k:RewriteContext A B) (g:DD B) 
-  (rs:RewriteState e k g)
-  : rewrite_context_interp e k ≃ g := rs.
+  {A B:WeakSetoid} (e:DD A) (k:RewriteContext A B) (g:DD B) 
+  : Type := k ⊛ e ≃ g.
 Opaque RewriteState.
-
-Definition rewrite_context_replace
-  {A B:WeakSetoid} 
-  (e:DD A) (e':DD A) (p:e ≃ e') (k:RewriteContext A B) (g:DD B) (rc:RewriteState e' k g)
-  : RewriteState e k g.
-Proof.
-  apply mk_RewriteState ; apply un_RewriteState in rc.
-  Transitivity (rewrite_context_interp e' k) ; auto.
-  apply rewrite_context_respect_weqv ; auto.
-Defined.
-
-Definition rewrite_context_elim {A:WeakSetoid} (e:DD A) (g:DD A) (rc:RewriteState e RCTop g) : e ≃ g.
-Proof.
-  apply un_RewriteState in rc ; simpl in * ; auto.
-Defined.
-
-Ltac Enter :=
-  match goal with
-  | [ |- ?x ≃ ?y ] => apply (rewrite_context_elim x y)
-  end.
-
-Ltac ReplaceBy q :=
-  try Enter ;
-  match goal with
-  | [ |- RewriteState ?e ?k ?g ] => apply (rewrite_context_replace e _ q k g)
-  end.
-
-Ltac ReplaceWith e' :=
-  try Enter ;
-  match goal with
-  | [ |- RewriteState ?e ?k ?g ] => 
-      let q := fresh "q" in
-      refine (let q := (_ : e ≈ e') in rewrite_context_replace e e' q k g _)
-  end.
 
 Module Notation.
   Notation "κ⊤" := RCTop.
@@ -97,3 +32,125 @@ Module Notation.
   Infix "▷" := RCFocusArg (at level 60, right associativity).
   Notation "【  f    ∈    c    ≃    g 】" := (RewriteState f c g).
 End Notation.
+Import Notation.
+
+Definition rewrite_state_enter 
+  {A:WeakSetoid} {e:DD A} {g:DD A} (p:RewriteState e κ⊤ g) 
+  : e ≃ g := p.
+Ltac Enter :=
+  match goal with
+  | [ |- ?e ≃ ?g ] => apply rewrite_state_enter
+  end.
+Ltac Enter0 :=
+  match goal with
+  | [ |- ?e ≃ ?g ] => change (RewriteState e κ⊤ g)
+  end.
+
+Definition rewrite_state_exit
+  {A:WeakSetoid} {e:DD A} {g:DD A} (p:e ≃ g) 
+  : RewriteState e RCTop g := p.
+Ltac Exit :=
+  match goal with
+  | [ |- RewriteState ?e RCTop ?g ] => apply rewrite_state_exit
+  end.
+Ltac Exit0 :=
+  match goal with
+  | [ |- RewriteState ?e RCTop ?g ] => change (e ≃ g)
+  end.
+
+Definition rewrite_state_push_fun
+  {A B C:WeakSetoid} {f:DD (A ⇨ B)} {x:DD A} {k:RewriteContext B C} {g:DD C}
+  (p:RewriteState f (k ◁ x) g)
+  : RewriteState (f ⊛ x) k g := p.
+Ltac PushFun :=
+  match goal with
+  | [ |- RewriteState (?f ⊛ ?x) ?k ?g ] => apply rewrite_state_push_fun
+  end.
+Ltac PushFun0 :=
+  match goal with
+  | [ |- RewriteState (?f ⊛ ?x) ?k ?g ] => change (RewriteState f (k ◁ x) g)
+  end.
+
+Definition rewrite_state_push_arg
+  {A B C:WeakSetoid} {f:DD (A ⇨ B)} {x:DD A} {k:RewriteContext B C} {g:DD C}
+  (p:RewriteState x (k ▷ f) g)
+  : RewriteState (f ⊛ x) k g := p.
+Ltac PushArg :=
+  match goal with
+  | [ |- RewriteState (?f ⊛ ?x) ?k ?g ] => apply rewrite_state_push_arg
+  end.
+Ltac PushArg0 :=
+  match goal with
+  | [ |- RewriteState (?f ⊛ ?x) ?k ?g ] => change (RewriteState x (k ▷ f) g)
+  end.
+
+Definition rewrite_state_pop_fun
+  {A B C:WeakSetoid} {f:DD (A ⇨ B)} {x:DD A} {k:RewriteContext B C} {g:DD C}
+  (p:RewriteState (f ⊛ x) k g)
+  : RewriteState f (k ◁ x) g := p.
+Definition rewrite_state_pop_arg
+  {A B C:WeakSetoid} {f:DD (A ⇨ B)} {x:DD A} {k:RewriteContext B C} {g:DD C}
+  (p:RewriteState (f ⊛ x) k g)
+  : RewriteState x (k ▷ f) g := p.
+Ltac Pop :=
+  match goal with
+  | [ |- RewriteState ?f (?k ◁ ?x) ?g ] => apply rewrite_state_pop_fun
+  | [ |- RewriteState ?x (?k ▷ ?f) ?g ] => apply rewrite_state_pop_arg
+  end.
+Ltac Pop0 :=
+  match goal with
+  | [ |- RewriteState ?f (?k ◁ ?x) ?g ] => change (RewriteState (f ⊛ x) k g)
+  | [ |- RewriteState ?x (?k ▷ ?f) ?g ] => change (RewriteState (f ⊛ x) k g)
+  end.
+
+Ltac Escape := repeat Pop ; Exit.
+Ltac Swap := try Escape ; Symmetry ; try Enter.
+
+Definition rewrite_context_replace
+  {A B:WeakSetoid} 
+  {e:DD A} {e':DD A} (p:e ≃ e') {k:RewriteContext A B} {g:DD B} (rc:RewriteState e' k g)
+  : RewriteState e k g.
+Proof.
+  change (k ⊛ e ≃ g) ; change (k ⊛ e' ≃ g) in rc.
+  Transitivity (k ⊛ e') ; auto ; decide_weqv_beta.
+Defined.
+
+Ltac ReplaceBy q :=
+  match goal with
+  | [ |- RewriteState ?e ?k ?g ] => apply (rewrite_context_replace q)
+  end.
+
+Ltac ReplaceWith e' :=
+  match goal with
+  | [ |- RewriteState ?e ?k ?g ] => 
+      let q := fresh "q" in
+      refine (let q := (_ : e ≈ e') in rewrite_context_replace q _)
+  end.
+
+Ltac Everywhere_1 t :=
+  match goal with
+  | [ |- RewriteState (_ ⊛ _) _ _ ] =>
+    chain PushFun ; Everywhere_1 t ; Pop |+|
+    chain PushArg ; Everywhere_1 t ; Pop |+|
+    t ; repeat t
+  | _ => t ; repeat t
+  end.
+
+Ltac Everywhere t := 
+  try (Enter ; Everywhere_1 t ; Exit) ;
+  try (Symmetry ; Enter ; Everywhere_1 t ; Exit) ;
+  try Reflexivity.
+
+Ltac Everywhere_10 t :=
+  match goal with
+  | [ |- RewriteState (_ ⊛ _) _ _ ] =>
+    chain PushFun0 ; Everywhere_10 t ; Pop0 |+|
+    chain PushArg0 ; Everywhere_10 t ; Pop0 |+|
+    t ; repeat t
+  | _ => t ; repeat t
+  end.
+
+Ltac Everywhere0 t := 
+  try (Enter0 ; Everywhere_10 t ; Exit0) ;
+  try (Symmetry ; Enter0 ; Everywhere_10 t ; Exit0) ;
+  try Reflexivity.
