src/FP/Data/Tactic.v
@@ -1,0 +1,2 @@
+Tactic Notation "chain" tactic(t1) "|+|" tactic(t2) := ((t1 ; try t2) || t2).
+
